```Haskell
a -> (b -> c)
```
```swift
(A) -> ((B) -> C)
```
................
```Haskell
a -> b -> c
```
```swift
(A) -> (B) -> C
```
................
```Haskell
catstr :: String -> String -> String
catstr s s' = s ++ s'
```
```swift
func catstr(_ s1 : String, _ s2 : String) -> String {
  return s1 + s2
}á›Œ
```
................
```Haskell
catstr' s = \s' -> s ++ s'
```
```swift
func catstr2(_ s1 : String) -> (String) -> String {
  return { s2 in s1 + s2 }
}
```
................
```Haskell
greet :: String -> String
greet = catstr "Hello "
```
```swift
func greet(_ s : String) -> String {
  return catstr("Hello ", s)
}
```
................
```Haskell
(a, b) -> c
```
```swift
(A, B) -> C
```
................
```Haskell
curry :: ((a, b)->c) -> (a->b->c)
curry f a b = f (a, b)
```
```swift
func curry<A, B, C>(_ f : @escaping (A, B) -> C) -> (A) -> (B) -> C {
  return { a in { b in f(a, b) } }
}
```
................
```Haskell
uncurry :: (a->b->c) -> ((a, b)->c)
uncurry f (a, b) = f a b
```
```swift
func uncurry<A, B, C>(_ f : @escaping (A) -> (B) -> C) -> (A, B) -> C {
  return { a, b in f(a)(b) }
}
```
................
```Haskell
factorizer :: ((a, b)->c) -> (a->(b->c))
factorizer g = \a -> (\b -> g (a, b))
```
```swift
func factorizer<A, B, C>(_ g : @escaping (A, B) -> C) -> (A) -> ((B) -> C) {
  return { a in { b in g(a, b) } }
}
```
................
```Haskell
f :: Either Int Double -> String
```
```swift
func f(_ x : Either<Int, Double>) -> String
```
................
```Haskell
f (Left n)  = if n < 0 then "Negative int" else "Positive int"
f (Right x) = if x < 0.0 then "Negative double" else "Positive double"
```
```swift
func f(_ x : Either<Int, Double>) -> String {
  switch(x) {
    case is Left<Int, Double>:
      let value = (x as! Left<Int, Double>).a
      return (value < 0) ? "Negative int" : "Positive int"
    default:
      let value = (x as! Right<Int, Double>).b
      return (value < 0) ? "Negative double" : "Positive double"
  }
}
```
................
```Haskell
eval :: ((a -> b), a) -> b
```
```swift
func eval<A, B>(_ f : (A) -> B, _ a : A) -> B
```
................
```Haskell
eval :: ((a -> b), a) -> b
eval (f, x) = f x
```
```swift
func eval<A, B>(_ f : (A) -> B, _ a : A) -> B {
  return f(a)
}
```
................
```Haskell
Either a b -> a
```
```swift
Either<A, B> -> A
```
................
```Haskell
absurd :: Void -> a
```
```swift
func absurd<A>(_ x : Never) -> A
```
