```Haskell
p' = p . m
q' = q . m
```
```swift
let p_prime = compose(p, m)
let q_prime = compose(q, m)
```
...................
```Haskell
contramap :: (c' -> c) -> (c -> LimD) -> (c' -> LimD)
contramap f u = u . f
```
```tut:invisible
trait Lim[T[_]]
```
```swift
func contramap<C1, C2>(_ f : @escaping (C2) -> C1, _ u : @escaping (C1) -> LimD) -> (C2) -> LimD {
  return compose(u, f)
}
```
..................
```Haskell
f :: a -> b
g :: a -> b
```
```swift
func f<A, B>(_ a : A) -> B
func g<A, B>(_ a : A) -> B
```
..................
```Haskell
p :: c -> a
q :: c -> b
```
```swift
func p<C, A>(_ c : C) -> A
func q<C, B>(_ c : C) -> B
```
..................
```Haskell
q = f . p
q = g . p
```
```swift
q == compose(f, p)
q == compose(g, p)
```
..................
```Haskell
f . p = g . p
```
```swift
compose(f, p) == compose(g, p)
```
..................
```Haskell
f (x, y) = 2 * y + x
g (x, y) = y - x
```
```swift
func f(_ x : Int, _ y : Int) -> Int {
  return 2 * y + x
}

func g(_ x : Int, _ y : Int) -> Int {
  return y - x
}
```
..................
```Haskell
p t = (t, (-2) * t)
```
```swift
func p(_ t : Int) -> (Int, Int) {
  return (t, -2 * t)
}
```
..................
```Haskell
f . p' = g . p'
```
```swift
compose(f, p_prime) == compose(g, p_prime)
```
..................
```Haskell
p'() = (0, 0)
```
```swift
func p_prime() -> (Int, Int) {
  return (0, 0)
}
```
..................
```Haskell
p' = p . h
```
```swift
let p_prime = compose(p, h)
```
..................
```Haskell
h () = 0
```
```swift
let h = { _ in 0 }
```
..................
```Haskell
f :: a -> b
g :: c -> b
```
```swift
func f<A, B>(_ a : A) -> B
func g<C, B>(_ c : C) -> C
```
..................
```Haskell
p :: d -> a
q :: d -> c
r :: d -> b
```
```swift
func p<D, A>(_ d : D) -> A
func q<D, C>(_ d : D) -> C
func r<D, B>(_ d : D) -> B
```
..................
```Haskell
g . q = f . p
```
```swift
compose(g, q) == compose(f, p)
```
..................
```Haskell
f x = 1.23
```
```swift
let f = { _ in 1.23 }
```
..................
```Haskell
newtype ToString a = ToString (a -> String)
instance Contravariant ToString where
    contramap f (ToString g) = ToString (g . f)
```
```swift
class ToString<A> : Kind<ForToString, A> {
  let f : (A) -> String

  static func fix(_ value : Kind<ForToString, A>) -> ToString<A> {
    return value as! ToString<A>
  }

  init(_ f : @escaping (A) -> String) {
    self.f = f
  }
}

class ToStringContravariant : Contravariant {
  typealias F : ForToString

  func contramap<A, B>(_ fa : Kind<ForToString, A>, _ f : @escaping (B) -> A) -> Kind<ForToString, B> {
    let fixed = ToString<A>.fix(fa)
    return ToString<B>(compose(fixed.f, f))
  }
}
```
..................
```Haskell
ToString (Either b c) ~ (b -> String, c -> String)
```
```swift
ToString<Either<B, C>> ~ ((B) -> String, (C) -> String)
```
..................
```Haskell
r -> (a, b) ~ (r -> a, r -> b)
```
```swift
(R) -> (A, B) ~ ((R) -> A, (R) -> B)
```
