```Haskell
class Monoid m where
    mempty  :: m
    mappend :: m -> m -> m
```
```swift
protocol Monoid {
  associatedtype M

  var mempty : M { get }
  func mappend(_ a : M, _ b : M) -> M
}
```
................
```Haskell
instance Monoid [a] where
    mempty = []
    mappend = (++)
```
```swift
class ArrayMonoid<A> : Monoid {
  typealias M = [A]

  var mempty : [A] {
    return []
  }

  func mappend(_ a : [A], _ b : [A]) -> [A] {
    return a + b
  }
}
```
................
```Haskell
2 * 3 = 6
[2] ++ [3] = [2, 3] // not the same as [6]
```
```swift
2 * 3 == 6
[2] + [3] == [2, 3] // not the same as [6]
```
................
```Haskell
h (a * b) = h a * h b
```
```swift
h(a * b) == h(a) * h(b)
```
................
```Haskell
[2] ++ [3] = [2, 3]
```
```swift
[2] + [3] = [2, 3]
```
................
```Haskell
2 * 3 = 6
```
```swift
2 * 3 == 6
```
................
```Haskell
p :: x -> U m
```
```swift
func p<X, U, M>(_ x : X) -> Kind<U, M>
```
................
```Haskell
q :: x -> U n
```
```swift
func q<X, U, N>(_ x : X) -> Kind<U, N>
```
................
```Haskell
h :: m -> n
```
```swift
func h<M, N>(_ m : M) -> N
```
................
```Haskell
q = U h . p
```
```swift
let q = compose(lift(h), p)
```
................
```Haskell
h a * h e = h (a * e) = h a
```
```swift
h(a) * h(e) == h(a * e) == h(a)
```
