```Haskell
swap       :: (a,b) -> (b,a)
swap (a,b) = (b,a)
```
```swift
func swap<A, B>(_ x : (A, B)) -> (B, A) {
  let (a, b) = x
  return (b, a)
}
```
................
```Haskell
return :: d -> m d
```
```swift
func pure<D, M>(_ d : D) -> Kind<M, D>
```
................
```Haskell
extract :: w c -> c
```
```swift
func extract<C, W>(_ wc : Kind<W, C>) -> C
```
................
```Haskell
class (Functor f, Representable u) =>
      Adjunction f u | f -> u, u -> f where
  unit         :: a -> u (f a)
  counit       :: f (u a) -> a
```
```swift
open class Adjunction<F, U, FunctorF, RepresentableU> where
  FunctorF : Functor, FunctorF.F == F,
  RepresentableU : Representable, RepresentableU.F == U {

  let functor : FunctorF
  let representable : RepresentableU

  init(_ functor : FunctorF, _ representable : RepresentableU) {
    self.functor = functor
    self.representable = representable
  }

  func unit<A>(_ a : A) -> Kind<U, Kind<F, A>> {
    fatalError("Implement unit in subclasses")
  }

  func counit<A>(_ a : A) -> Kind<F, Kind<U, A>> -> A {
    fatalError("Implement counit in subclasses")
  }
}
```
................
```Haskell
class (Functor f, Representable u) =>
      Adjunction f u | f -> u, u -> f where
  leftAdjunct  :: (f a -> b) -> (a -> u b)
  rightAdjunct :: (a -> u b) -> (f a -> b)
```
```swift
open class Adjunction<F, U, FunctorF, RepresentableU> where
  FunctorF : Functor, FuntorF.F == F,
  RepresentableU : Representable, RepresentableU.F == U {

  let functor : FunctorF
  let representable : RepresentableU

  init(_ functor : FunctorF, _ representable : RepresentableU) {
    self.functor = functor
    self.representable = representable
  }

  func leftAdjunct<A, B>(_ a : A, _ f : @escaping (Kind<F, A>) -> B) -> Kind<U, B> {
    fatalError("Implement leftAdjunct in subclasses")
  }

  func rightAdjunct<A, B>(_ fa : Kind<F, A>, _ f : @escaping (A) -> Kind<U, B>) -> B {
    fatalError("Implement rightAdjunct in subclasses")
  }
}
```
................
```Haskell
  unit           = leftAdjunct id
  counit         = rightAdjunct id
  leftAdjunct f  = fmap f . unit
  rightAdjunct f = counit . fmap f
```
```swift
func unit<A>(_ a : A) -> Kind<U, Kind<F, A>> {
  return leftAdjunct(a, id)
}

func counit<A>(_ a : Kind<U, Kind<F, A>>) -> A {
  return rightAdjunct(a, id)
}

func leftAdjunt<A, B>(_ a : A, _ f : @escaping (Kind<F, A>) -> B) -> Kind<U, B> {
  return representable.map(unit(a), f)
}

func rightAdjunct<A, B>(_ a : Kind<F, A>, _ f : @escaping (A) -> Kind<U, B>) -> B {
  return counit(functor.map(a, f))
}
```
................
```Haskell
factorizer :: (c -> a) -> (c -> b) -> (c -> (a, b))
factorizer p q = \x -> (p x, q x)
```
```swift
func factorizer<A, B, C>(_ p : @escaping (C) -> A, _ q : @escaping (C) -> B) -> (C) -> (A, B) {
  return { x in (p(x), q(x)) }
}
```
................
```Haskell
fst . factorizer p q = p
snd . factorizer p q = q
```
```swift
andThen(factorizer(p, q), { c in c.0 }) == p
andThen(factorizer(p, q), { c in c.1 }) == q
```
................
```Haskell
(,) Int Bool ~ (Int, Bool)
```
```swift
Tuple<Int, Bool> ~ (Int, Bool)
```
